\chapter{Appendix}

\section{Integration of Growth Model} \label{sec:substitution}

Integrate using substitution:

\begin{eqnarray*}
\frac{dN}{dt}                                &=& kNln\left(\frac{M}{N} \right) \\
\frac{dN}{Nln\left(\frac{M}{N} \right)}      &=& kdt \\
\int \frac{dN}{Nln\left(\frac{M}{N} \right)} &=& \int kdt \\
\end{eqnarray*}

\begin{align*}
\text{with}\ u &= ln\left(\frac{M}{N} \right) & \text{and}\ && \frac{du}{dN} &= -\frac{1}{N}
\end{align*}
% dN = -Ndu \]

\begin{eqnarray*}
\int \frac{-Ndu}{Nu} &=& \int kdt \\
\int -\frac{1}{u}du &=& \int kdt \\
-ln\left(|{u}| \right) &=& kt + c \\
ln\left(|{u}| \right) &=& -kt - c \\
ln\left(\left|\ln\left(\dfrac{M}{N}\right)\right|\right) &=& -kt - c \\
ln\left(\dfrac{M}{N}\right) &=& e^{-kt - c} \\
\dfrac{M}{N}                &=& e^{e^{-kt - c}} \\
N                           &=& \dfrac{M}{e^{e^{-kt - c}}}
\end{eqnarray*}


\clearpage

Calculate c using the initial values provided:

\begin{align*}
    M &= 10^{13} & k &= 0.06 & N &= 10^9 & t &= 0
\end{align*}

\begin{eqnarray*}
10^9        &=& \dfrac{10^{13}}{e^{e^{-0.006(0) - c}}} \\
e^{e^{-c}}  &=& \dfrac{10^{13}}{10^9} \\
e^{e^{-c}}  &=& {10^4} \\
-c          &=& ln\left(\left|\ln\left({10^4}\right)\right|\right) \\
c           &=& -ln\left(\left|\ln\left({10^4}\right)\right|\right) \\
\end{eqnarray*}

Substitute c back into the equation and simplify:

\begin{eqnarray*}
N &=& \dfrac{M}{e^{e^{-kt + ln\left(\left|\ln\left({10^4}\right)\right|\right)}}} \\
  &=& \dfrac{M}{e^{e^{-kt} e^{ln\left(\left|\ln\left({10^4}\right)\right|\right)}}} \\
  &=& \dfrac{M}{e^{e^{-kt} \ln\left({10^4}\right)}} \\
  &=& \dfrac{M}{(e^{\ln\left({10^4}\right)})^{e^{-kt}}} \\
N  &=& \dfrac{M}{10^{4e^{-kt}}}
\end{eqnarray*}

\clearpage